src/hls/Veriloggenproof.v
@@ -22,247 +22,247 @@ From vericert Require HTL.
 From vericert Require Import Vericertlib Veriloggen Verilog ValueInt AssocMap.
 Require Import Lia.
 
-
 Local Open Scope assocmap.
 
 Definition match_prog (prog : HTL.program) (tprog : Verilog.program) :=
   match_program (fun cu f tf => Errors.OK tf = transl_fundef prog f) eq prog tprog.
 
-(*
-
 Lemma transf_program_match:
-  forall prog, match_prog prog (transl_program prog).
+  forall prog tprog, transl_program prog = Errors.OK tprog -> match_prog prog tprog.
 Proof.
-  intros. eapply match_transform_program_contextual. auto.
+  intros. unfold transl_program in *. eapply match_transform_partial_program_contextual; eauto.
 Qed.
 
-Inductive match_stacks : list HTL.stackframe -> list stackframe -> Prop :=
-| match_stack :
-    forall res m pc reg_assoc arr_assoc hstk vstk,
-      match_stacks hstk vstk ->
-      match_stacks (HTL.Stackframe res m pc reg_assoc arr_assoc :: hstk)
-                   (Stackframe res (transl_module m) pc
-                                       reg_assoc arr_assoc :: vstk)
-| match_stack_nil : match_stacks nil nil.
+Instance TransfVerilogLink : TransfLink Veriloggenproof.match_prog.
+Admitted.
 
-Inductive match_states : HTL.state -> state -> Prop :=
-| match_state :
-    forall m st reg_assoc arr_assoc hstk vstk,
-      match_stacks hstk vstk ->
-      match_states (HTL.State hstk m st reg_assoc arr_assoc)
-                   (State vstk (transl_module m) st reg_assoc arr_assoc)
-| match_returnstate :
-    forall v hstk vstk,
-      match_stacks hstk vstk ->
-      match_states (HTL.Returnstate hstk v) (Returnstate vstk v)
-| match_initial_call :
-    forall m,
-      match_states (HTL.Callstate nil m nil) (Callstate nil (transl_module m) nil).
+(* Inductive match_stacks : list HTL.stackframe -> list stackframe -> Prop := *)
+(* | match_stack : *)
+(*     forall res m pc reg_assoc arr_assoc hstk vstk, *)
+(*       match_stacks hstk vstk -> *)
+(*       match_stacks (HTL.Stackframe res m pc reg_assoc arr_assoc :: hstk) *)
+(*                    (Stackframe res (transl_module m) pc *)
+(*                                        reg_assoc arr_assoc :: vstk) *)
+(* | match_stack_nil : match_stacks nil nil. *)
 
-Lemma Vlit_inj :
-  forall a b, Vlit a = Vlit b -> a = b.
-Proof. inversion 1. trivial. Qed.
+(* Inductive match_states : HTL.state -> state -> Prop := *)
+(* | match_state : *)
+(*     forall m st reg_assoc arr_assoc hstk vstk, *)
+(*       match_stacks hstk vstk -> *)
+(*       match_states (HTL.State hstk m st reg_assoc arr_assoc) *)
+(*                    (State vstk (transl_module m) st reg_assoc arr_assoc) *)
+(* | match_returnstate : *)
+(*     forall v hstk vstk, *)
+(*       match_stacks hstk vstk -> *)
+(*       match_states (HTL.Returnstate hstk v) (Returnstate vstk v) *)
+(* | match_initial_call : *)
+(*     forall m, *)
+(*       match_states (HTL.Callstate nil m nil) (Callstate nil (transl_module m) nil). *)
 
-Lemma posToValue_inj :
-  forall a b,
-    0 <= Z.pos a <= Int.max_unsigned ->
-    0 <= Z.pos b <= Int.max_unsigned ->
-    posToValue a = posToValue b ->
-    a = b.
-Proof.
-  intros. rewrite <- Pos2Z.id at 1. rewrite <- Pos2Z.id.
-  rewrite <- Int.unsigned_repr at 1; try assumption.
-  symmetry.
-  rewrite <- Int.unsigned_repr at 1; try assumption.
-  unfold posToValue in *. rewrite H1; auto.
-Qed.
+(* Lemma Vlit_inj : *)
+(*   forall a b, Vlit a = Vlit b -> a = b. *)
+(* Proof. inversion 1. trivial. Qed. *)
 
-Lemma valueToPos_inj :
-  forall a b,
-    0 < Int.unsigned a ->
-    0 < Int.unsigned b ->
-    valueToPos a = valueToPos b ->
-    a = b.
-Proof.
-  intros. unfold valueToPos in *.
-  rewrite <- Int.repr_unsigned at 1.
-  rewrite <- Int.repr_unsigned.
-  apply Pos2Z.inj_iff in H1.
-  rewrite Z2Pos.id in H1; auto.
-  rewrite Z2Pos.id in H1; auto.
-  rewrite H1. auto.
-Qed.
+(* Lemma posToValue_inj : *)
+(*   forall a b, *)
+(*     0 <= Z.pos a <= Int.max_unsigned -> *)
+(*     0 <= Z.pos b <= Int.max_unsigned -> *)
+(*     posToValue a = posToValue b -> *)
+(*     a = b. *)
+(* Proof. *)
+(*   intros. rewrite <- Pos2Z.id at 1. rewrite <- Pos2Z.id. *)
+(*   rewrite <- Int.unsigned_repr at 1; try assumption. *)
+(*   symmetry. *)
+(*   rewrite <- Int.unsigned_repr at 1; try assumption. *)
+(*   unfold posToValue in *. rewrite H1; auto. *)
+(* Qed. *)
 
-Lemma unsigned_posToValue_le :
-  forall p,
-    Z.pos p <= Int.max_unsigned ->
-    0 < Int.unsigned (posToValue p).
-Proof.
-  intros. unfold posToValue. rewrite Int.unsigned_repr; lia.
-Qed.
+(* Lemma valueToPos_inj : *)
+(*   forall a b, *)
+(*     0 < Int.unsigned a -> *)
+(*     0 < Int.unsigned b -> *)
+(*     valueToPos a = valueToPos b -> *)
+(*     a = b. *)
+(* Proof. *)
+(*   intros. unfold valueToPos in *. *)
+(*   rewrite <- Int.repr_unsigned at 1. *)
+(*   rewrite <- Int.repr_unsigned. *)
+(*   apply Pos2Z.inj_iff in H1. *)
+(*   rewrite Z2Pos.id in H1; auto. *)
+(*   rewrite Z2Pos.id in H1; auto. *)
+(*   rewrite H1. auto. *)
+(* Qed. *)
 
-Lemma transl_ctrl_fun_fst :
-  forall p1 p2 a b,
-    0 <= Z.pos p1 <= Int.max_unsigned ->
-    0 <= Z.pos p2 <= Int.max_unsigned ->
-    transl_ctrl_fun (p1, a) = transl_ctrl_fun (p2, b) ->
-    (p1, a) = (p2, b).
-Proof.
-  intros. unfold transl_ctrl_fun in H1. apply pair_equal_spec in H1.
-  destruct H1. rewrite H2. apply Vlit_inj in H1.
-  apply posToValue_inj in H1; try assumption.
-  rewrite H1; auto.
-Qed.
+(* Lemma unsigned_posToValue_le : *)
+(*   forall p, *)
+(*     Z.pos p <= Int.max_unsigned -> *)
+(*     0 < Int.unsigned (posToValue p). *)
+(* Proof. *)
+(*   intros. unfold posToValue. rewrite Int.unsigned_repr; lia. *)
+(* Qed. *)
 
-Lemma transl_data_fun_fst :
-  forall p1 p2 a b,
-    0 <= Z.pos p1 <= Int.max_unsigned ->
-    0 <= Z.pos p2 <= Int.max_unsigned ->
-    transl_datapath_fun (p1, a) = transl_datapath_fun (p2, b) ->
-    p1 = p2.
-Proof.
-  intros.
-  unfold transl_datapath_fun in H1. apply pair_equal_spec in H1. destruct H1.
-  apply Vlit_inj in H1. apply posToValue_inj in H1; assumption.
-Qed.
+(* Lemma transl_ctrl_fun_fst : *)
+(*   forall p1 p2 a b, *)
+(*     0 <= Z.pos p1 <= Int.max_unsigned -> *)
+(*     0 <= Z.pos p2 <= Int.max_unsigned -> *)
+(*     transl_ctrl_fun (p1, a) = transl_ctrl_fun (p2, b) -> *)
+(*     (p1, a) = (p2, b). *)
+(* Proof. *)
+(*   intros. unfold transl_ctrl_fun in H1. apply pair_equal_spec in H1. *)
+(*   destruct H1. rewrite H2. apply Vlit_inj in H1. *)
+(*   apply posToValue_inj in H1; try assumption. *)
+(*   rewrite H1; auto. *)
+(* Qed. *)
 
-Lemma Zle_relax :
-  forall p q r,
-  p < q <= r ->
-  p <= q <= r.
-Proof. lia. Qed.
-Hint Resolve Zle_relax : verilogproof.
+(* Lemma transl_data_fun_fst : *)
+(*   forall p1 p2 a b, *)
+(*     0 <= Z.pos p1 <= Int.max_unsigned -> *)
+(*     0 <= Z.pos p2 <= Int.max_unsigned -> *)
+(*     transl_datapath_fun (p1, a) = transl_datapath_fun (p2, b) -> *)
+(*     p1 = p2. *)
+(* Proof. *)
+(*   intros. *)
+(*   unfold transl_datapath_fun in H1. apply pair_equal_spec in H1. destruct H1. *)
+(*   apply Vlit_inj in H1. apply posToValue_inj in H1; assumption. *)
+(* Qed. *)
 
-Lemma transl_in :
-  forall l p,
-  0 <= Z.pos p <= Int.max_unsigned ->
-  (forall p0, In p0 (List.map fst l) -> 0 < Z.pos p0 <= Int.max_unsigned) ->
-  In (Vlit (posToValue p)) (map fst (map transl_ctrl_fun l)) ->
-  In p (map fst l).
-Proof.
-  induction l.
-  - simplify. auto.
-  - intros. destruct a. simplify. destruct (peq p0 p); auto.
-    right. inv H1. apply Vlit_inj in H. apply posToValue_inj in H; auto. contradiction.
-    auto with verilogproof.
-    apply IHl; auto.
-Qed.
+(* Lemma Zle_relax : *)
+(*   forall p q r, *)
+(*   p < q <= r -> *)
+(*   p <= q <= r. *)
+(* Proof. lia. Qed. *)
+(* Hint Resolve Zle_relax : verilogproof. *)
 
-Lemma transl_notin :
-  forall l p,
-    0 <= Z.pos p <= Int.max_unsigned ->
-    (forall p0, In p0 (List.map fst l) -> 0 < Z.pos p0 <= Int.max_unsigned) ->
-    ~ In p (List.map fst l) -> ~ In (Vlit (posToValue p)) (List.map fst (transl_ctrl l)).
-Proof.
-  induction l; auto. intros. destruct a. unfold not in *. intros.
-  simplify.
-  destruct (peq p0 p). apply H1. auto. apply H1.
-  unfold transl_ctrl in *. inv H2. apply Vlit_inj in H. apply posToValue_inj in H.
-  contradiction.
-  auto with verilogproof. auto.
-  right. apply transl_in; auto.
-Qed.
+(* Lemma transl_in : *)
+(*   forall l p, *)
+(*   0 <= Z.pos p <= Int.max_unsigned -> *)
+(*   (forall p0, In p0 (List.map fst l) -> 0 < Z.pos p0 <= Int.max_unsigned) -> *)
+(*   In (Vlit (posToValue p)) (map fst (map transl_ctrl_fun l)) -> *)
+(*   In p (map fst l). *)
+(* Proof. *)
+(*   induction l. *)
+(*   - simplify. auto. *)
+(*   - intros. destruct a. simplify. destruct (peq p0 p); auto. *)
+(*     right. inv H1. apply Vlit_inj in H. apply posToValue_inj in H; auto. contradiction. *)
+(*     auto with verilogproof. *)
+(*     apply IHl; auto. *)
+(* Qed. *)
 
-Lemma transl_norepet :
-  forall l,
-    (forall p0, In p0 (List.map fst l) -> 0 < Z.pos p0 <= Int.max_unsigned) ->
-    list_norepet (List.map fst l) -> list_norepet (List.map fst (transl_ctrl l)).
-Proof.
-  induction l.
-  - intros. simpl. apply list_norepet_nil.
-  - destruct a. intros. simpl. apply list_norepet_cons.
-    inv H0. apply transl_notin. apply Zle_relax. apply H. simplify; auto.
-    intros. apply H. destruct (peq p0 p); subst; simplify; auto.
-    assumption. apply IHl. intros. apply H. destruct (peq p0 p); subst; simplify; auto.
-    simplify. inv H0. assumption.
-Qed.
+(* Lemma transl_notin : *)
+(*   forall l p, *)
+(*     0 <= Z.pos p <= Int.max_unsigned -> *)
+(*     (forall p0, In p0 (List.map fst l) -> 0 < Z.pos p0 <= Int.max_unsigned) -> *)
+(*     ~ In p (List.map fst l) -> ~ In (Vlit (posToValue p)) (List.map fst (transl_ctrl l)). *)
+(* Proof. *)
+(*   induction l; auto. intros. destruct a. unfold not in *. intros. *)
+(*   simplify. *)
+(*   destruct (peq p0 p). apply H1. auto. apply H1. *)
+(*   unfold transl_ctrl in *. inv H2. apply Vlit_inj in H. apply posToValue_inj in H. *)
+(*   contradiction. *)
+(*   auto with verilogproof. auto. *)
+(*   right. apply transl_in; auto. *)
+(* Qed. *)
 
-Lemma transl_ctrl_correct :
-  forall l v ev f asr asa asrn asan asr' asa' asrn' asan',
-    (forall p0, In p0 (List.map fst l) -> 0 < Z.pos p0 <= Int.max_unsigned) ->
-    list_norepet (List.map fst l) ->
-    asr!ev = Some v ->
-    (forall p s,
-        In (p, s) l ->
-        v = posToValue p ->
-        stmnt_runp f
-                   {| assoc_blocking := asr; assoc_nonblocking := asrn |}
-                   {| assoc_blocking := asa; assoc_nonblocking := asan |}
-                   s
-                   {| assoc_blocking := asr'; assoc_nonblocking := asrn' |}
-                   {| assoc_blocking := asa'; assoc_nonblocking := asan' |} ->
-        stmnt_runp f
-                   {| assoc_blocking := asr; assoc_nonblocking := asrn |}
-                   {| assoc_blocking := asa; assoc_nonblocking := asan |}
-                   (Vcase (Vvar ev) (transl_ctrl l) (Some Vskip))
-                   {| assoc_blocking := asr'; assoc_nonblocking := asrn' |}
-                   {| assoc_blocking := asa'; assoc_nonblocking := asan' |}).
-Proof.
-  induction l as [| a l IHl].
-  - contradiction.
-  - intros v ev f asr asa asrn asan asr' asa' asrn' asan' BOUND NOREP ASSOC p s IN EQ SRUN.
-    destruct a as [p' s']. simplify.
-    destruct (peq p p'); subst. eapply stmnt_runp_Vcase_match.
-    constructor. simplify. unfold AssocMap.find_assocmap, AssocMapExt.get_default.
-    rewrite ASSOC. trivial. constructor. auto.
-    inversion IN as [INV | INV]. inversion INV as [INV2]; subst. assumption.
-    inv NOREP. eapply in_map with (f := fst) in INV. contradiction.
+(* Lemma transl_norepet : *)
+(*   forall l, *)
+(*     (forall p0, In p0 (List.map fst l) -> 0 < Z.pos p0 <= Int.max_unsigned) -> *)
+(*     list_norepet (List.map fst l) -> list_norepet (List.map fst (transl_ctrl l)). *)
+(* Proof. *)
+(*   induction l. *)
+(*   - intros. simpl. apply list_norepet_nil. *)
+(*   - destruct a. intros. simpl. apply list_norepet_cons. *)
+(*     inv H0. apply transl_notin. apply Zle_relax. apply H. simplify; auto. *)
+(*     intros. apply H. destruct (peq p0 p); subst; simplify; auto. *)
+(*     assumption. apply IHl. intros. apply H. destruct (peq p0 p); subst; simplify; auto. *)
+(*     simplify. inv H0. assumption. *)
+(* Qed. *)
 
-    eapply stmnt_runp_Vcase_nomatch. constructor. simplify.
-    unfold AssocMap.find_assocmap, AssocMapExt.get_default. rewrite ASSOC.
-    trivial. constructor. unfold not. intros. apply n. apply posToValue_inj.
-    apply Zle_relax. apply BOUND. right. inv IN. inv H0; contradiction.
-    eapply in_map with (f := fst) in H0. auto.
-    apply Zle_relax. apply BOUND; auto. auto.
+(* Lemma transl_ctrl_correct : *)
+(*   forall l v ev f asr asa asrn asan asr' asa' asrn' asan', *)
+(*     (forall p0, In p0 (List.map fst l) -> 0 < Z.pos p0 <= Int.max_unsigned) -> *)
+(*     list_norepet (List.map fst l) -> *)
+(*     asr!ev = Some v -> *)
+(*     (forall p s, *)
+(*         In (p, s) l -> *)
+(*         v = posToValue p -> *)
+(*         stmnt_runp f *)
+(*                    {| assoc_blocking := asr; assoc_nonblocking := asrn |} *)
+(*                    {| assoc_blocking := asa; assoc_nonblocking := asan |} *)
+(*                    s *)
+(*                    {| assoc_blocking := asr'; assoc_nonblocking := asrn' |} *)
+(*                    {| assoc_blocking := asa'; assoc_nonblocking := asan' |} -> *)
+(*         stmnt_runp f *)
+(*                    {| assoc_blocking := asr; assoc_nonblocking := asrn |} *)
+(*                    {| assoc_blocking := asa; assoc_nonblocking := asan |} *)
+(*                    (Vcase (Vvar ev) (transl_ctrl l) (Some Vskip)) *)
+(*                    {| assoc_blocking := asr'; assoc_nonblocking := asrn' |} *)
+(*                    {| assoc_blocking := asa'; assoc_nonblocking := asan' |}). *)
+(* Proof. *)
+(*   induction l as [| a l IHl]. *)
+(*   - contradiction. *)
+(*   - intros v ev f asr asa asrn asan asr' asa' asrn' asan' BOUND NOREP ASSOC p s IN EQ SRUN. *)
+(*     destruct a as [p' s']. simplify. *)
+(*     destruct (peq p p'); subst. eapply stmnt_runp_Vcase_match. *)
+(*     constructor. simplify. unfold AssocMap.find_assocmap, AssocMapExt.get_default. *)
+(*     rewrite ASSOC. trivial. constructor. auto. *)
+(*     inversion IN as [INV | INV]. inversion INV as [INV2]; subst. assumption. *)
+(*     inv NOREP. eapply in_map with (f := fst) in INV. contradiction. *)
 
-    eapply IHl. auto. inv NOREP. auto. eassumption. inv IN. inv H. contradiction. apply H.
-    trivial. assumption.
-Qed.
-Hint Resolve transl_ctrl_correct : verilogproof.
+(*     eapply stmnt_runp_Vcase_nomatch. constructor. simplify. *)
+(*     unfold AssocMap.find_assocmap, AssocMapExt.get_default. rewrite ASSOC. *)
+(*     trivial. constructor. unfold not. intros. apply n. apply posToValue_inj. *)
+(*     apply Zle_relax. apply BOUND. right. inv IN. inv H0; contradiction. *)
+(*     eapply in_map with (f := fst) in H0. auto. *)
+(*     apply Zle_relax. apply BOUND; auto. auto. *)
 
-(* FIXME Probably wrong we probably need some statemnt about datapath_statement_runp *)
-Lemma transl_datapath_correct :
-  forall l v ev f asr asa asrn asan asr' asa' asrn' asan',
-    (forall p0, In p0 (List.map fst l) -> 0 < Z.pos p0 <= Int.max_unsigned) ->
-    list_norepet (List.map fst l) ->
-    asr!ev = Some v ->
-    (forall p s,
-        In (p, s) l ->
-        v = posToValue p ->
-        stmnt_runp f
-                   {| assoc_blocking := asr; assoc_nonblocking := asrn |}
-                   {| assoc_blocking := asa; assoc_nonblocking := asan |}
-                   s
-                   {| assoc_blocking := asr'; assoc_nonblocking := asrn' |}
-                   {| assoc_blocking := asa'; assoc_nonblocking := asan' |} ->
-        stmnt_runp f
-                   {| assoc_blocking := asr; assoc_nonblocking := asrn |}
-                   {| assoc_blocking := asa; assoc_nonblocking := asan |}
-                   (Vcase (Vvar ev) (transl_ctrl l) (Some Vskip))
-                   {| assoc_blocking := asr'; assoc_nonblocking := asrn' |}
-                   {| assoc_blocking := asa'; assoc_nonblocking := asan' |}).
-Proof. Admitted.
+(*     eapply IHl. auto. inv NOREP. auto. eassumption. inv IN. inv H. contradiction. apply H. *)
+(*     trivial. assumption. *)
+(* Qed. *)
+(* Hint Resolve transl_ctrl_correct : verilogproof. *)
 
-Lemma pc_wf :
-  forall A m p v,
-  (forall p0, In p0 (List.map fst (@AssocMap.elements A m)) -> 0 < Z.pos p0 <= Int.max_unsigned) ->
-  m!p = Some v ->
-  0 <= Z.pos p <= Int.max_unsigned.
-Proof.
-  intros A m p v LT S. apply Zle_relax. apply LT.
-  apply AssocMap.elements_correct in S. remember (p, v) as x.
-  exploit in_map. apply S. instantiate (1 := fst). subst. simplify. auto.
-Qed.
+(* (* FIXME Probably wrong we probably need some statemnt about datapath_statement_runp *) *)
+(* Lemma transl_datapath_correct : *)
+(*   forall l v ev f asr asa asrn asan asr' asa' asrn' asan', *)
+(*     (forall p0, In p0 (List.map fst l) -> 0 < Z.pos p0 <= Int.max_unsigned) -> *)
+(*     list_norepet (List.map fst l) -> *)
+(*     asr!ev = Some v -> *)
+(*     (forall p s, *)
+(*         In (p, s) l -> *)
+(*         v = posToValue p -> *)
+(*         stmnt_runp f *)
+(*                    {| assoc_blocking := asr; assoc_nonblocking := asrn |} *)
+(*                    {| assoc_blocking := asa; assoc_nonblocking := asan |} *)
+(*                    s *)
+(*                    {| assoc_blocking := asr'; assoc_nonblocking := asrn' |} *)
+(*                    {| assoc_blocking := asa'; assoc_nonblocking := asan' |} -> *)
+(*         stmnt_runp f *)
+(*                    {| assoc_blocking := asr; assoc_nonblocking := asrn |} *)
+(*                    {| assoc_blocking := asa; assoc_nonblocking := asan |} *)
+(*                    (Vcase (Vvar ev) (transl_ctrl l) (Some Vskip)) *)
+(*                    {| assoc_blocking := asr'; assoc_nonblocking := asrn' |} *)
+(*                    {| assoc_blocking := asa'; assoc_nonblocking := asan' |}). *)
+(* Proof. Admitted. *)
 
-Lemma mis_stepp_decl :
-  forall l asr asa f,
-    mis_stepp f asr asa (map Vdeclaration l) asr asa.
-Proof.
-  induction l.
-  - intros. constructor.
-  - intros. simplify. econstructor. constructor. auto.
-Qed.
-Hint Resolve mis_stepp_decl : verilogproof.
+(* Lemma pc_wf : *)
+(*   forall A m p v, *)
+(*   (forall p0, In p0 (List.map fst (@AssocMap.elements A m)) -> 0 < Z.pos p0 <= Int.max_unsigned) -> *)
+(*   m!p = Some v -> *)
+(*   0 <= Z.pos p <= Int.max_unsigned. *)
+(* Proof. *)
+(*   intros A m p v LT S. apply Zle_relax. apply LT. *)
+(*   apply AssocMap.elements_correct in S. remember (p, v) as x. *)
+(*   exploit in_map. apply S. instantiate (1 := fst). subst. simplify. auto. *)
+(* Qed. *)
+
+(* Lemma mis_stepp_decl : *)
+(*   forall l asr asa f, *)
+(*     mis_stepp f asr asa (map Vdeclaration l) asr asa. *)
+(* Proof. *)
+(*   induction l. *)
+(*   - intros. constructor. *)
+(*   - intros. simplify. econstructor. constructor. auto. *)
+(* Qed. *)
+(* Hint Resolve mis_stepp_decl : verilogproof. *)
 
 Section CORRECTNESS.
 
@@ -279,133 +279,133 @@ Section CORRECTNESS.
   Proof. intros. eapply (Genv.find_symbol_match TRANSL). Qed.
   Hint Resolve symbols_preserved : verilogproof.
 
-  Lemma function_ptr_translated:
-    forall (b: Values.block) (f: HTL.fundef),
-      Genv.find_funct_ptr ge b = Some f ->
-      exists tf,
-        Genv.find_funct_ptr tge b = Some tf /\ transl_fundef f = tf.
-  Proof.
-    intros. exploit (Genv.find_funct_ptr_match TRANSL); eauto.
-    intros (cu & tf & P & Q & R); exists tf; auto.
-  Qed.
-  Hint Resolve function_ptr_translated : verilogproof.
+(*   Lemma function_ptr_translated: *)
+(*     forall (b: Values.block) (f: HTL.fundef), *)
+(*       Genv.find_funct_ptr ge b = Some f -> *)
+(*       exists tf, *)
+(*         Genv.find_funct_ptr tge b = Some tf /\ transl_fundef f = tf. *)
+(*   Proof. *)
+(*     intros. exploit (Genv.find_funct_ptr_match TRANSL); eauto. *)
+(*     intros (cu & tf & P & Q & R); exists tf; auto. *)
+(*   Qed. *)
+(*   Hint Resolve function_ptr_translated : verilogproof. *)
 
-  Lemma functions_translated:
-    forall (v: Values.val) (f: HTL.fundef),
-      Genv.find_funct ge v = Some f ->
-      exists tf,
-        Genv.find_funct tge v = Some tf /\ transl_fundef f = tf.
-  Proof.
-    intros. exploit (Genv.find_funct_match TRANSL); eauto.
-    intros (cu & tf & P & Q & R); exists tf; auto.
-  Qed.
-  Hint Resolve functions_translated : verilogproof.
+(*   Lemma functions_translated: *)
+(*     forall (v: Values.val) (f: HTL.fundef), *)
+(*       Genv.find_funct ge v = Some f -> *)
+(*       exists tf, *)
+(*         Genv.find_funct tge v = Some tf /\ transl_fundef f = tf. *)
+(*   Proof. *)
+(*     intros. exploit (Genv.find_funct_match TRANSL); eauto. *)
+(*     intros (cu & tf & P & Q & R); exists tf; auto. *)
+(*   Qed. *)
+(*   Hint Resolve functions_translated : verilogproof. *)
 
-  Lemma senv_preserved:
-    Senv.equiv (Genv.to_senv ge) (Genv.to_senv tge).
-  Proof.
-    intros. eapply (Genv.senv_match TRANSL).
-  Qed.
-  Hint Resolve senv_preserved : verilogproof.
+(*   Lemma senv_preserved: *)
+(*     Senv.equiv (Genv.to_senv ge) (Genv.to_senv tge). *)
+(*   Proof. *)
+(*     intros. eapply (Genv.senv_match TRANSL). *)
+(*   Qed. *)
+(*   Hint Resolve senv_preserved : verilogproof. *)
 
-  Theorem transl_step_correct :
-    forall (S1 : HTL.state) t S2,
-      HTL.step ge S1 t S2 ->
-      forall (R1 : state),
-        match_states S1 R1 ->
-        exists R2, Smallstep.plus step tge R1 t R2 /\ match_states S2 R2.
-  Proof.
-    induction 1; intros R1 MSTATE; inv MSTATE.
-    - econstructor; split. apply Smallstep.plus_one. econstructor.
-      assumption. assumption. eassumption. apply valueToPos_posToValue.
-      split. lia.
-      eapply pc_wf. intros. pose proof (HTL.mod_wf m) as HP. destruct HP as [HP _].
-      split. lia. apply HP. eassumption. eassumption.
-      econstructor. econstructor. eapply stmnt_runp_Vcond_false. econstructor. econstructor.
-      simpl. unfold find_assocmap. unfold AssocMapExt.get_default.
-      rewrite H. trivial.
+(*   Theorem transl_step_correct : *)
+(*     forall (S1 : HTL.state) t S2, *)
+(*       HTL.step ge S1 t S2 -> *)
+(*       forall (R1 : state), *)
+(*         match_states S1 R1 -> *)
+(*         exists R2, Smallstep.plus step tge R1 t R2 /\ match_states S2 R2. *)
+(*   Proof. *)
+(*     induction 1; intros R1 MSTATE; inv MSTATE. *)
+(*     - econstructor; split. apply Smallstep.plus_one. econstructor. *)
+(*       assumption. assumption. eassumption. apply valueToPos_posToValue. *)
+(*       split. lia. *)
+(*       eapply pc_wf. intros. pose proof (HTL.mod_wf m) as HP. destruct HP as [HP _]. *)
+(*       split. lia. apply HP. eassumption. eassumption. *)
+(*       econstructor. econstructor. eapply stmnt_runp_Vcond_false. econstructor. econstructor. *)
+(*       simpl. unfold find_assocmap. unfold AssocMapExt.get_default. *)
+(*       rewrite H. trivial. *)
 
-      econstructor. simpl. auto. auto.
+(*       econstructor. simpl. auto. auto. *)
 
-      eapply transl_ctrl_correct.
-      intros. split. lia. pose proof (HTL.mod_wf m) as HP. destruct HP as [HP _]. auto.
-      apply Maps.PTree.elements_keys_norepet. eassumption.
-      2: { apply valueToPos_inj. apply unsigned_posToValue_le.
-           eapply pc_wf. intros. pose proof (HTL.mod_wf m) as HP. destruct HP as [HP _].
-           split. lia. apply HP. eassumption. eassumption.
-           apply unsigned_posToValue_le. eapply pc_wf. intros. pose proof (HTL.mod_wf m) as HP.
-           destruct HP as [HP _].
-           split. lia. apply HP. eassumption. eassumption. trivial.
-      }
-      apply Maps.PTree.elements_correct. eassumption. eassumption.
+(*       eapply transl_ctrl_correct. *)
+(*       intros. split. lia. pose proof (HTL.mod_wf m) as HP. destruct HP as [HP _]. auto. *)
+(*       apply Maps.PTree.elements_keys_norepet. eassumption. *)
+(*       2: { apply valueToPos_inj. apply unsigned_posToValue_le. *)
+(*            eapply pc_wf. intros. pose proof (HTL.mod_wf m) as HP. destruct HP as [HP _]. *)
+(*            split. lia. apply HP. eassumption. eassumption. *)
+(*            apply unsigned_posToValue_le. eapply pc_wf. intros. pose proof (HTL.mod_wf m) as HP. *)
+(*            destruct HP as [HP _]. *)
+(*            split. lia. apply HP. eassumption. eassumption. trivial. *)
+(*       } *)
+(*       apply Maps.PTree.elements_correct. eassumption. eassumption. *)
 
-      econstructor. econstructor.
+(*       econstructor. econstructor. *)
 
-      { admit.
-      (*
-      eapply transl_list_correct.
-      intros. split. lia. pose proof (HTL.mod_wf m) as HP. destruct HP as [_ HP]. auto.
-      apply Maps.PTree.elements_keys_norepet. eassumption.
-      2: { apply valueToPos_inj. apply unsigned_posToValue_le.
-           eapply pc_wf. intros. pose proof (HTL.mod_wf m) as HP. destruct HP as [HP _].
-           split. lia. apply HP. eassumption. eassumption.
-           apply unsigned_posToValue_le. eapply pc_wf. intros. pose proof (HTL.mod_wf m) as HP.
-           destruct HP as [HP _].
-           split. lia. apply HP. eassumption. eassumption. trivial.
-      }
-      apply Maps.PTree.elements_correct. eassumption. eassumption.
-      *)
-      }
+(*       { admit. *)
+(*       (* *) *)
+(* (*       eapply transl_list_correct. *) *)
+(* (*       intros. split. lia. pose proof (HTL.mod_wf m) as HP. destruct HP as [_ HP]. auto. *) *)
+(* (*       apply Maps.PTree.elements_keys_norepet. eassumption. *) *)
+(* (*       2: { apply valueToPos_inj. apply unsigned_posToValue_le. *) *)
+(* (*            eapply pc_wf. intros. pose proof (HTL.mod_wf m) as HP. destruct HP as [HP _]. *) *)
+(* (*            split. lia. apply HP. eassumption. eassumption. *) *)
+(* (*            apply unsigned_posToValue_le. eapply pc_wf. intros. pose proof (HTL.mod_wf m) as HP. *) *)
+(* (*            destruct HP as [HP _]. *) *)
+(* (*            split. lia. apply HP. eassumption. eassumption. trivial. *) *)
+(* (*       } *) *)
+(* (*       apply Maps.PTree.elements_correct. eassumption. eassumption. *) *)
+(* (*       *) *)
+(*       } *)
 
-      apply mis_stepp_decl. trivial. trivial. simpl. eassumption. auto.
-      rewrite valueToPos_posToValue. constructor; assumption. lia.
-    - econstructor; split. apply Smallstep.plus_one. apply step_finish. assumption. eassumption.
-      constructor; assumption.
-    - econstructor; split. apply Smallstep.plus_one. constructor.
+(*       apply mis_stepp_decl. trivial. trivial. simpl. eassumption. auto. *)
+(*       rewrite valueToPos_posToValue. constructor; assumption. lia. *)
+(*     - econstructor; split. apply Smallstep.plus_one. apply step_finish. assumption. eassumption. *)
+(*       constructor; assumption. *)
+(*     - econstructor; split. apply Smallstep.plus_one. constructor. *)
 
-      constructor. constructor.
-    - inv H3. econstructor; split. apply Smallstep.plus_one. constructor. trivial.
+(*       constructor. constructor. *)
+(*     - inv H3. econstructor; split. apply Smallstep.plus_one. constructor. trivial. *)
 
-      apply match_state. assumption.
-  Admitted.
-  Hint Resolve transl_step_correct : verilogproof.
+(*       apply match_state. assumption. *)
+(*   Admitted. *)
+(*   Hint Resolve transl_step_correct : verilogproof. *)
 
-  Lemma transl_initial_states :
-    forall s1 : Smallstep.state (HTL.semantics prog),
-      Smallstep.initial_state (HTL.semantics prog) s1 ->
-      exists s2 : Smallstep.state (Verilog.semantics tprog),
-        Smallstep.initial_state (Verilog.semantics tprog) s2 /\ match_states s1 s2.
-  Proof.
-    induction 1.
-    econstructor; split. econstructor.
-    apply (Genv.init_mem_transf TRANSL); eauto.
-    rewrite symbols_preserved.
-    replace (AST.prog_main tprog) with (AST.prog_main prog); eauto.
-    symmetry; eapply Linking.match_program_main; eauto.
-    exploit function_ptr_translated; eauto. intros [tf [A B]].
-    inv B. eauto.
-    constructor.
-  Qed.
-  Hint Resolve transl_initial_states : verilogproof.
+(*   Lemma transl_initial_states : *)
+(*     forall s1 : Smallstep.state (HTL.semantics prog), *)
+(*       Smallstep.initial_state (HTL.semantics prog) s1 -> *)
+(*       exists s2 : Smallstep.state (Verilog.semantics tprog), *)
+(*         Smallstep.initial_state (Verilog.semantics tprog) s2 /\ match_states s1 s2. *)
+(*   Proof. *)
+(*     induction 1. *)
+(*     econstructor; split. econstructor. *)
+(*     apply (Genv.init_mem_transf TRANSL); eauto. *)
+(*     rewrite symbols_preserved. *)
+(*     replace (AST.prog_main tprog) with (AST.prog_main prog); eauto. *)
+(*     symmetry; eapply Linking.match_program_main; eauto. *)
+(*     exploit function_ptr_translated; eauto. intros [tf [A B]]. *)
+(*     inv B. eauto. *)
+(*     constructor. *)
+(*   Qed. *)
+(*   Hint Resolve transl_initial_states : verilogproof. *)
 
-  Lemma transl_final_states :
-    forall (s1 : Smallstep.state (HTL.semantics prog))
-           (s2 : Smallstep.state (Verilog.semantics tprog))
-           (r : Integers.Int.int),
-      match_states s1 s2 ->
-      Smallstep.final_state (HTL.semantics prog) s1 r ->
-      Smallstep.final_state (Verilog.semantics tprog) s2 r.
-  Proof.
-    intros. inv H0. inv H. inv H3. constructor. reflexivity.
-  Qed.
-  Hint Resolve transl_final_states : verilogproof.
+(*   Lemma transl_final_states : *)
+(*     forall (s1 : Smallstep.state (HTL.semantics prog)) *)
+(*            (s2 : Smallstep.state (Verilog.semantics tprog)) *)
+(*            (r : Integers.Int.int), *)
+(*       match_states s1 s2 -> *)
+(*       Smallstep.final_state (HTL.semantics prog) s1 r -> *)
+(*       Smallstep.final_state (Verilog.semantics tprog) s2 r. *)
+(*   Proof. *)
+(*     intros. inv H0. inv H. inv H3. constructor. reflexivity. *)
+(*   Qed. *)
+(*   Hint Resolve transl_final_states : verilogproof. *)
 
   Theorem transf_program_correct:
     forward_simulation (HTL.semantics prog) (Verilog.semantics tprog).
   Proof.
-    eapply Smallstep.forward_simulation_plus; eauto with verilogproof.
-    apply senv_preserved.
-  Qed.
+    (* eapply Smallstep.forward_simulation_plus; eauto with verilogproof. *)
+    (* apply senv_preserved. *)
+    admit.
+  Admitted.
 
 End CORRECTNESS.
-*)
